theories/ValueOpts/Eqn.v
@@ -832,3 +832,32 @@ Proof.
   intuition; eapply unsatisfiables_Proper_impl; eauto;
     rewrite H; eauto.
 Qed.
+
+Lemma satisfies_single E gamma
+  : satisfies E gamma
+    -> satisfiesAll E {gamma}.
+Proof.
+  intros; hnf; intros.
+  cset_tac'. rewrite <- H0; eauto.
+Qed.
+
+Lemma satisfies_single' E gamma
+  : satisfiesAll E {gamma}
+    -> satisfies E gamma.
+Proof.
+  intros. eapply H. cset_tac.
+Qed.
+
+Lemma satisfies_add_extr E gamma Gamma
+  : satisfiesAll E {gamma; Gamma}
+    -> satisfies E gamma.
+Proof.
+  intros. eapply H. cset_tac.
+Qed.
+
+Lemma satisfies_add_drop E gamma Gamma
+  : satisfiesAll E {gamma; Gamma}
+    -> satisfiesAll E Gamma.
+Proof.
+  intros. hnf; intros. eapply H. cset_tac.
+Qed.
